wip: expose loop_inv, as_seq, gsub

lib/Lib.Buffer.fsti
@@ -3,8 +3,6 @@ module Lib.Buffer
 open FStar.HyperStack
 open FStar.HyperStack.ST
 
-open LowStar.Buffer
-
 open Lib.IntTypes
 open Lib.RawIntTypes
 
@@ -28,14 +26,23 @@ val length: #a:Type0 -> b:buffer a -> GTot (r:size_nat{r == B.length b})
 let lbuffer (a:Type0) (len:size_nat) = b:buffer a {length b == len}
 let lbytes len = lbuffer uint8 len
 
-val gsub:
+inline_for_extraction
+val as_seq:
     #a:Type0
   -> #len:size_nat
-  -> #olen:size_nat
+  -> h:mem
   -> b:lbuffer a len
-  -> start:size_t
-  -> n:size_t{v start + v n <= len /\ v n == olen}
-  -> GTot (lbuffer a olen)
+  -> GTot (s:Seq.seq a{s == B.as_seq h b}) //Seq.length s == len
+
+let gsub
+    (#a:Type0)
+    (#len:size_nat)
+    (#olen:size_nat)
+    (b:lbuffer a len)
+    (start:size_t)
+    (n:size_t{v start + v n <= len /\ v n == olen}) //: GTot (lbuffer a olen)
+ =
+  B.gsub b (size_to_UInt32 start) (size_to_UInt32 n)
 
 inline_for_extraction
 val sub:
@@ -47,7 +54,7 @@ val sub:
   -> n:size_t{v start + v n <= len /\ v n == olen}
   -> Stack (lbuffer a olen)
     (requires fun h0 -> B.live h0 b)
-    (ensures  fun h0 r h1 -> h0 == h1 /\ r == B.gsub b (size_to_UInt32 start) (size_to_UInt32 n))
+    (ensures  fun h0 r h1 -> h0 == h1 /\ r == gsub #a #len #olen b start n)
 
 inline_for_extraction
 val index:
@@ -57,7 +64,7 @@ val index:
   -> i:size_t{v i < len}
   -> Stack a
     (requires fun h0 -> B.live h0 b)
-    (ensures  fun h0 r h1 -> h0 == h1 /\ r == Seq.index #a #len (B.as_seq h1 b) (v i))
+    (ensures  fun h0 r h1 -> h0 == h1 /\ r == Seq.index #a #len (as_seq h1 b) (v i))
 
 inline_for_extraction
 val upd:
@@ -69,15 +76,14 @@ val upd:
   -> Stack unit
     (requires fun h0 -> B.live h0 b)
     (ensures  fun h0 _ h1 ->
-      modifies (loc_buffer b) h0 h1 /\ B.live h1 b /\
-      B.as_seq h1 b == Seq.upd #a #len (B.as_seq h0 b) (v i) x)
+      B.modifies (B.loc_buffer b) h0 h1 /\ B.live h1 b /\
+      as_seq h1 b == Seq.upd #a #len (as_seq h0 b) (v i) x)
 
 inline_for_extraction let op_Array_Assignment #a #len = upd #a #len
 
 inline_for_extraction let op_Array_Access #a #len = index #a #len
 
-unfold
-let bget #a #n h (b:lbuffer a n) i = Seq.index #_ #n (B.as_seq h b) i
+let bget (#a:Type0) (#len:size_nat) h (b:lbuffer a len) i = Seq.index #a #len (as_seq h b) i
 
 inline_for_extraction
 val create:
@@ -89,7 +95,7 @@ val create:
     (requires fun h0 -> len > 0)
     (ensures  fun h0 b h1 ->
       B.alloc_post_mem_common b h0 h1 (Seq.create len init) /\
-      frameOf b = HS.get_tip h0)
+      B.frameOf b = HS.get_tip h0)
 
 inline_for_extraction noextract
 val createL:
@@ -98,8 +104,8 @@ val createL:
   -> StackInline (lbuffer a (normalize_term (List.Tot.length init)))
     (requires fun h0 -> B.alloca_of_list_pre #a init)
     (ensures fun h0 b h1 ->
-      alloc_post_mem_common b h0 h1 (Seq.of_list init) /\
-      frameOf b = HS.get_tip h0)
+      B.alloc_post_mem_common b h0 h1 (Seq.of_list init) /\
+      B.frameOf b = HS.get_tip h0)
 
 inline_for_extraction
 val recall:
@@ -115,7 +121,7 @@ val createL_global:
     #a:Type0
   -> init:list a{List.Tot.length init <= max_size_t}
   -> ST (b:lbuffer a (normalize_term (List.Tot.length init)){
-    frameOf b == HyperStack.root /\ recallable b})
+    B.frameOf b == HyperStack.root /\ B.recallable b})
     (requires fun h0 -> B.gcmalloc_of_list_pre #a HyperStack.root init)
     (ensures  fun h0 b h1 ->
       B.alloc_post_mem_common b h0 h1 (Seq.of_list init))
@@ -130,8 +136,8 @@ val copy:
   -> Stack unit
     (requires fun h0 -> B.live h0 o /\ B.live h0 i /\ B.disjoint i o)
     (ensures  fun h0 _ h1 ->
-      B.live h1 o /\ B.live h1 i /\ modifies (loc_buffer o) h0 h1 /\
-      B.as_seq h1 o == B.as_seq h0 i)
+      B.live h1 o /\ B.live h1 i /\ B.modifies (B.loc_buffer o) h0 h1 /\
+      as_seq h1 o == as_seq h0 i)
 
 inline_for_extraction
 val update_sub:
@@ -143,8 +149,8 @@ val update_sub:
   -> src:lbuffer a (size_v n)
   -> Stack unit
     (requires fun h -> B.live h dst /\ B.live h src /\ B.disjoint dst src)
-    (ensures  fun h0 _ h1 -> B.live h1 dst /\ modifies (loc_buffer dst) h0 h1 /\
-      B.as_seq h1 dst == Seq.update_sub #a #len (B.as_seq h0 dst) (v start) (v n) (B.as_seq h0 src))
+    (ensures  fun h0 _ h1 -> B.live h1 dst /\ B.modifies (B.loc_buffer dst) h0 h1 /\
+      as_seq h1 dst == Seq.update_sub #a #len (as_seq h0 dst) (v start) (v n) (as_seq h0 src))
 
 (** Loop combinator with just memory safety specification *)
 inline_for_extraction noextract
@@ -156,11 +162,11 @@ val loop_nospec:
   -> buf:lbuffer a len
   -> impl:
       (i:size_t{v i < v n} -> Stack unit
-        (requires fun h -> modifies (loc_buffer buf) h0 h)
-        (ensures  fun _ _ h1 -> modifies (loc_buffer buf) h0 h1))
+        (requires fun h -> B.modifies (B.loc_buffer buf) h0 h)
+        (ensures  fun _ _ h1 -> B.modifies (B.loc_buffer buf) h0 h1))
   -> Stack unit
     (requires fun h -> h0 == h /\ B.live h0 buf)
-    (ensures  fun _ _ h1 -> modifies (loc_buffer buf) h0 h1)
+    (ensures  fun _ _ h1 -> B.modifies (B.loc_buffer buf) h0 h1)
 
 (**
 * A generalized loop combinator paremetrized by its state (e.g. an accumulator)
@@ -176,18 +182,20 @@ val loop_nospec:
 * - [impl] the body of the loop as a Stack function
 *)
 inline_for_extraction noextract
-val loop_inv:
-    h0:mem
-  -> n:size_t
-  -> a_spec:(i:size_nat{i <= v n} -> Type)
-  -> a_impl:Type
-  -> acc:a_impl
-  -> refl:(mem -> i:size_nat{i <= v n} -> GTot (a_spec i))
-  -> footprint:(i:size_nat{i <= v n} -> GTot loc)
-  -> spec:(mem -> GTot (i:size_nat{i < v n} -> a_spec i -> a_spec (i + 1)))
-  -> i:size_nat{i <= v n}
-  -> h:mem
-  -> Type0
+let loop_inv
+    (h0:mem)
+    (n:size_t)
+    (a_spec:(i:size_nat{i <= v n} -> Type))
+    (a_impl:Type)
+    (acc:a_impl)
+    (refl:(mem -> i:size_nat{i <= v n} -> GTot (a_spec i)))
+    (footprint:(i:size_nat{i <= v n} -> GTot B.loc))
+    (spec:(mem -> GTot (i:size_nat{i < v n} -> a_spec i -> a_spec (i + 1))))
+    (i:size_nat{i <= v n})
+    (h:mem) : Type0
+ =
+  B.modifies (footprint i) h0 h /\
+  refl h i == Seq.repeat i a_spec (spec h0) (refl h0 0)
 
 inline_for_extraction noextract
 val loop:
@@ -197,7 +205,7 @@ val loop:
   -> a_impl:Type
   -> acc:a_impl
   -> refl:(mem -> i:size_nat{i <= v n} -> GTot (a_spec i))
-  -> footprint:(i:size_nat{i <= v n} -> GTot loc)
+  -> footprint:(i:size_nat{i <= v n} -> GTot B.loc)
   -> spec:(mem -> GTot (i:size_nat{i < v n} -> a_spec i -> a_spec (i + 1)))
   -> impl:(i:size_t{v i < v n} -> Stack unit
      (requires loop_inv h0 n a_spec a_impl acc refl footprint spec (v i))
@@ -207,16 +215,18 @@ val loop:
     (ensures  fun _ _ -> loop_inv h0 n a_spec a_impl acc refl footprint spec (v n))
 
 inline_for_extraction noextract
-val loop1_inv:
-    h0:mem
-  -> n:size_t
-  -> b: Type
-  -> blen: size_nat
-  -> acc:lbuffer b blen
-  -> spec:(mem -> GTot (i:size_nat{i < v n} -> Seq.lseq b blen -> Seq.lseq b blen))
-  -> i:size_nat{i <= v n}
-  -> h:mem
-  -> Type0
+let loop1_inv
+    (h0:mem)
+    (n:size_t)
+    (b: Type)
+    (blen: size_nat)
+    (acc:lbuffer b blen)
+    (spec:(mem -> GTot (i:size_nat{i < v n} -> Seq.lseq b blen -> Seq.lseq b blen)))
+    (i:size_nat{i <= v n})
+    (h:mem) : Type0
+ =
+  B.modifies (B.loc_buffer acc) h0 h /\
+  as_seq h acc == Seq.repeati i (spec h0) (as_seq h0 acc)
 
 inline_for_extraction noextract
 val loop1:
@@ -240,9 +250,9 @@ val lbytes_eq:
   -> a:lbuffer uint8 (v len)
   -> b:lbuffer uint8 (v len)
   -> Stack bool
-    (requires fun h -> live h a /\ live h b)
+    (requires fun h -> B.live h a /\ B.live h b)
     (ensures  fun h0 r h1 ->
-      modifies loc_none h0 h1 /\
+      B.modifies B.loc_none h0 h1 /\
       r == Seq.lbytes_eq #(v len) (as_seq h0 a) (as_seq h0 b))
 
 inline_for_extraction
@@ -259,12 +269,12 @@ val alloc:
   -> spec:(h:mem -> GTot(r:b -> Seq.lseq w wlen -> Type))
   -> impl:(buf:lbuffer a len ->
     Stack b
-      (requires (fun h -> modifies (loc_buffer buf) h0 h /\ live h0 write))
-      (ensures (fun h r h' -> modifies (loc_union (loc_buffer buf) (loc_buffer write)) h h' /\
+      (requires (fun h -> B.modifies (B.loc_buffer buf) h0 h /\ B.live h0 write))
+      (ensures (fun h r h' -> B.modifies (B.loc_union (B.loc_buffer buf) (B.loc_buffer write)) h h' /\
 			                  spec h0 r (as_seq h' write)))) ->
   Stack b
-    (requires (fun h -> h == h0 /\ live h write))
-    (ensures (fun h0 r h1 -> modifies (loc_buffer write) h0 h1 /\
+    (requires (fun h -> h == h0 /\ B.live h write))
+    (ensures (fun h0 r h1 -> B.modifies (B.loc_buffer write) h0 h1 /\
 		                    spec h0 r (as_seq h1 write)))
 
 // TODO: used in tests; move to a different module
